minor cleaning (#26)

examples/airlock.v
@@ -32,20 +32,14 @@ Context {Fx : effect} `{DOORS -< Fx} {M : freerMonad Fx}.
 Definition is_open d : M bool := ptrigger $ CheckOpen d.
 Definition toggle d : M unit := ptrigger $ Toggle d.
 Definition open_door d : M unit :=
-  is_open d >>= fun open => when (~~ open) (toggle d).
+  is_open d >>= fun b => when (~~ b) (toggle d).
 Definition close_door d : M unit :=
-  is_open d >>= (when ^~ (toggle d)).
+  is_open d >>= fun b => when b (toggle d).
 End doors_s.
 
 Inductive CONTROLLER : effect :=
 | Tick : CONTROLLER unit
-| TriggerOpen d : CONTROLLER unit.
-
-Section controller_s.
-Context {Fx : effect} `{CONTROLLER -< Fx} {M : freerMonad Fx}.
-Definition tick : M unit := ptrigger Tick.
-Definition trigger_open d : M unit := ptrigger $ TriggerOpen d.
-End controller_s.
+| PressButton d : CONTROLLER unit.
 
 Definition opposite_door d : door :=
   match d with
@@ -53,20 +47,17 @@ Definition opposite_door d : door :=
   | right => left
   end.
 
-Lemma co_leftE : opposite_door left = right.
-Proof. by []. Qed.
-
 Definition controller {Fx : effect} `{DOORS -< Fx, STORE nat -< Fx}
     {M : freerMonad Fx} : component (M := M) CONTROLLER Fx :=
   fun _ op =>
     match op with
     | Tick =>
       iget >>= fun cpt =>
-      when (15 <? cpt)%nat $
+      when (15 < cpt)%N $
         close_door left >>
         close_door right >>
         iput 0%nat
-    | TriggerOpen d =>
+    | PressButton d =>
       close_door (opposite_door d) >>
       open_door d >>
       iput 0%nat
@@ -75,32 +66,28 @@ End DoorsControllerM.
 
 (** * Verifying the Airlock Controller *)
 
-(** ** Doors Specification *)
-
-(* ----------------------------- Witness States ----------------------------- *)
-
 Definition open := true.
 Definition closed := false.
 
-Definition Ω : Type := bool * bool.
+Definition state : Type := bool * bool.
 
-Definition door_state d : Ω -> bool :=
+Definition door_state d : state -> bool :=
   match d with
   | left => fst
   | right => snd
   end.
 
-Definition toggle d (t : Ω) : Ω :=
+Definition toggle d (t : state) : state :=
   match d with
   | left => (~~ t.1, t.2)
   | right => (t.1, ~~ t.2)
   end.
 
-Lemma tog_equ_1 d (ω : Ω) :
+Lemma tog_equ_1 d (ω : state) :
   door_state d (toggle d ω) = ~~ door_state d ω.
 Proof. by case: d. Qed.
 
-Lemma tog_equ_2 d (ω : Ω) :
+Lemma tog_equ_2 d (ω : state) :
   door_state (opposite_door d) (toggle d ω) = door_state (opposite_door d) ω.
 Proof. by case: d. Qed.
 
@@ -117,20 +104,20 @@ Opaque toggle.
     trick to prevent [cbn] to unfold impure computations covered by intermediary
     theorems. *)
 
-(* -------------------------------- Contract -------------------------------- *)
-(* Ω = bool * bool : doors state *)
-Definition doors_witness_update (t : Ω) (U : Type) (c : DOORS U) : Ω :=
-  if c is Toggle d then toggle d t else t.
+Section contract.
+Implicit Types s : state.
 
-(** *** Requirements / Precondition *)
-Definition doors_requirement (t : Ω) : forall U, DOORS U -> Prop :=
+Definition doors_witness_update s (U : Type) (c : DOORS U) : state :=
+  if c is Toggle d then toggle d s else s.
+
+Definition doors_requirement s : forall U, DOORS U -> Prop :=
   fun _ op =>
-     match op with
-     | CheckOpen _ => True
-     | Toggle d => door_state (opposite_door d) t -> door_state d t
-     end.
+    match op with
+    | CheckOpen _ => True
+    | Toggle d => door_state (opposite_door d) s -> door_state d s
+    end.
 (*
-doors_o_caller does not hold when we toggle a door d
+doors_requirement does not hold when we toggle a door d
 which is closed while the opposite door is open;
 observe that doors_o_caller can be true if the opposite door is
 open while we try to close the other open door (though this
@@ -144,12 +131,10 @@ false false true
 false true  true
 *)
 
-(** *** Promises / PostCondition *)
-
-Definition doors_promise (t : Ω) : forall U, DOORS U -> U -> Prop :=
+Definition doors_promise s : forall U, DOORS U -> U -> Prop :=
   fun U op =>
     match op in DOORS _ with
-    | CheckOpen d => fun b => door_state d t = b
+    | CheckOpen d => fun b => door_state d s = b
     | Toggle _ => fun _ => True
     end.
 
@@ -158,24 +143,25 @@ relation between a command c and a state u;
 it is false only when the state of a door that we check is not u
 *)
 
-
-(* doors_c => {{door_caller}} p%step {{door_callee}} *)
-Definition doors_c : contract DOORS Ω :=
+Definition doors_c : contract DOORS state :=
   make_contract
    (fun t u c _ => doors_witness_update t u c)
    doors_requirement
    doors_promise.
 
+End contract.
+
 Local Open Scope classical_set_scope.
 
-Remark one_door_safe_all_doors_safe (ω : Ω) d
-    (safe : ~~ door_state d ω \/ ~~ door_state (opposite_door d) ω) :
-  forall d', ~~ door_state d' ω \/ ~~ door_state (opposite_door d') ω.
+Remark one_door_safe_all_doors_safe (ω : state) d
+    (safe : (~~ door_state d ω) || (~~ door_state (opposite_door d) ω)) :
+  forall d',(~~ door_state d' ω) || (~~ door_state (opposite_door d') ω).
 Proof.
-by move: d safe=> + /[swap]; case; case=> //=; rewrite or_comm.
+by move=> d'; move: d d' safe => [|] [|]//=; rewrite orbC.
 Qed.
 
-Definition doors_safe (ω : Ω) := ~~ door_state left ω \/ ~~ door_state right ω.
+Definition not_both_open s :=
+  (~~ door_state left s) || (~~ door_state right s).
 
 Section RespectfulAndRunLemmas.
 Context {Fx : effect} `{DOORS -< Fx} {M : freerMonad Fx}.
@@ -190,7 +176,7 @@ case=> w'; rewrite pre_to_hoare_whenP // !to_hoare_triggerE.
 by case=> ->; apply: provided_bind_caller=> /=.
 Qed.
 
-Lemma open_door_respectful (ω : Ω) d (safe : ~~ door_state (opposite_door d) ω) :
+Lemma open_door_respectful (ω : state) d (safe : ~~ door_state (opposite_door d) ω) :
   pre (doors_c |> (open_door d : M _)) ω.
 Proof.
 rewrite /open_door freer_to_hoare_bindE; split.
@@ -199,7 +185,7 @@ case=> w'; rewrite pre_to_hoare_whenP // !to_hoare_triggerE.
 by case=> ->; apply: provided_bind_caller; move: safe=> /= /negPf ->.
 Qed.
 
-Lemma close_door_run (ω : Ω) d (ω' : Ω) (x : unit)
+Lemma close_door_run (ω : state) d (ω' : state) (x : unit)
     (run : post (doors_c |> (close_door d : M _)) ω x ω') :
   ~~ door_state d ω'.
 Proof.
@@ -217,24 +203,24 @@ Opaque Nat.ltb.
 Opaque door_state.
 
 Lemma doors_trigger_preserves_safe
-    {a : Type} (op : Fx a) (ω : Ω) (x : a) (ω' : Ω) :
+    {a : Type} (op : Fx a) (ω : state) (x : a) (ω' : state) :
   pre (doors_c |> (ptrigger op : M _)) ω ->
   post (doors_c |> (ptrigger op : M _)) ω x ω' ->
-  doors_safe ω -> doors_safe ω'.
+  not_both_open ω -> not_both_open ω'.
 Proof.
 rewrite to_hoare_triggerE /=.
 rewrite /gen_requirement /gen_state_update /gen_promise.
-case: prj=> [door_op |] /=;
-  last by move=> _ [-> _].
+case: prj=> [door_op |_ [-> _ //]] /=.
 move: door_op x; case=> d /= [] caller [-> _] _ //.
 apply: (one_door_safe_all_doors_safe (toggle d ω) d).
+move: caller.
 rewrite tog_equ_1 tog_equ_2 negbK.
-case other_open: (door_state (opposite_door d) ω); [left | by right].
-by apply: caller; rewrite other_open.
+case: (door_state (opposite_door _)) => /=; rewrite ?orbF ?orbT//.
+exact.
 Qed.
 
 Lemma doors_handler_preserves_safe {a : Type} (op : Fx a) :
-  preserves_invariant doors_safe (hoare_of_contract doors_c op).
+  preserves_invariant not_both_open (hoare_of_contract doors_c op).
 Proof.
 move=> witness result witness' hpre hpost.
 apply: doors_trigger_preserves_safe;
@@ -242,6 +228,7 @@ apply: doors_trigger_preserves_safe;
 - exact: hpre.
 - exact: hpost.
 Qed.
+
 End RespectfulAndRunLemmas.
 
 (* From now on, proofs will use the inductive version. *)
@@ -253,18 +240,18 @@ Context {Fx : effect} `{DOORS -< Fx} {M : inductiveFreerMonad Fx}.
   * if the invariant was preserved all along.
   *)
 Lemma doors_run_preserves_safe {A : Type} (p : M A) :
-  preserves_invariant doors_safe (doors_c |> p).
+  preserves_invariant not_both_open (doors_c |> p).
 Proof.
 by apply: to_hoare_preserves_invariant=> *;
   exact: (doors_handler_preserves_safe (M := M)).
 Qed.
 
 Lemma respectful_run_inv {A : Type} (p : M A)
-    (ω : Ω) (safe : doors_safe ω)
-    (a : A) (ω' : Ω)
+    (ω : state) (safe : not_both_open ω)
+    (a : A) (ω' : state)
     (hpre : pre (doors_c |> p) ω)
     (hpost : post (doors_c |> p) ω a ω') :
-  doors_safe ω'.
+  not_both_open ω'.
 Proof. by move: hpre hpost safe; exact: doors_run_preserves_safe. Qed.
 End InvariantRunLemmas.
 
@@ -273,25 +260,23 @@ Section controller_s.
 Context {Fx : effect} `{DOORS ;; (STORE nat) -<< Fx}
   {M : inductiveFreerMonad Fx}.
 
-Lemma controller_pre {α : Type} (op : CONTROLLER α) (ω : Ω) :
-  pre (doors_c |> controller (M := M) α op) ω.
+Lemma controller_pre {A : Type} (op : CONTROLLER A) (ω : state) :
+  pre (doors_c |> controller (M := M) A op) ω.
 Proof.
-case: op=> [| d].
-- (* Tick *)
-  rewrite freer_to_hoare_bindE; split =>[|cpt w].
+case: op => [| d].
+- rewrite freer_to_hoare_bindE; split =>[|cpt w].
   + rewrite to_hoare_triggerE.
     exact: distinguished_caller.
-  + rewrite !to_hoare_triggerE.
+  + rewrite to_hoare_triggerE.
     move/distinguished_callee=> ->.
     rewrite pre_to_hoare_whenP.
-    case: (15 <? cpt)%nat=> //=.
+    case: (15 < cpt)%N => //=.
     rewrite freer_to_hoare_bindE; split => [|*].
     * by rewrite freer_to_hoare_bindE; split => [|*];
         rewrite close_door_respectful.
     * rewrite to_hoare_triggerE => x ?.
       by apply: distinguished_caller.
-- (* Trigger Open *)
-  rewrite freer_to_hoare_bindE; split => [|*].
+- rewrite freer_to_hoare_bindE; split => [|*].
   + rewrite freer_to_hoare_bindE; split => [|? ? close_post].
     * by rewrite close_door_respectful.
     * exact/open_door_respectful/close_door_run/close_post.
@@ -301,7 +286,7 @@ Qed.
 
 Theorem controller_correct :
   correct_component controller (M := M)
-    (no_contract CONTROLLER) doors_c (fun _ => doors_safe).
+    (no_contract CONTROLLER) doors_c (fun=> not_both_open).
 Proof.
 move=> ? ω ? ? op _; split=> [| ? ? hpost].
   exact: controller_pre.
